theories/L6_PCPS/toplevel_theorems.v
@@ -5,8 +5,10 @@ Require Import Coq.NArith.BinNat Coq.Relations.Relations Coq.MSets.MSets Coq.MSe
 Require Import L6.cps L6.eval L6.cps_util L6.identifiers L6.ctx L6.set_util
         L6.Ensembles_util L6.List_util L6.size_cps L6.tactics L6.relations L6.rel_comp
         L6.uncurry L6.bounds
-        L6.closure_conversion L6.closure_conversion_util L6.hoisting.
+        L6.closure_conversion L6.closure_conversion_util L6.hoisting
+        L6.lambda_lifting L6.lambda_lifting_correct.
 Require Export L6.logical_relations L6.logical_relations_cc L6.alpha_conv L6.inline_letapp L6.inline L6.inline_correct.
+Require Import Common.compM.
 Require Import compcert.lib.Coqlib.
 
 Import ListNotations.
@@ -35,11 +37,10 @@ Definition post_prop P1 PG :=
 
 Section Inline.
 
- Lemma inline_correct St IH e d st c :
+ Lemma inline_correct St IH e d st c z :
    well_scoped e ->
-   max_var e 1 < state.next_var c ->
    exists (e' : exp) (c' : state.comp_data),
-     beta_contract_top St IH e d st c true = (compM.Ret e', c') /\
+     inline_top St IH z e d st c true = (Ret e', c') /\
      wf_pres e e' /\
      max_var e' 1 < state.next_var c' /\
      (forall (k : nat) (rho1 rho2 : env),
@@ -48,8 +49,7 @@ Section Inline.
  Proof.
    intros.
    edestruct inline_correct_top with (P1 := fun L => inline_bound L d)
-                                     (PG := inline_bound d d).
-   
+                                     (PG := inline_bound d d).   
    - intros. eapply inline_bound_compat. eassumption.
    - intros. eapply inline_bound_post_Eapp_l.
    - intros. eapply inline_bound_remove_steps_letapp.
@@ -58,7 +58,6 @@ Section Inline.
    - eapply inline_bound_top_impl.
    - eapply H.
    - eapply H.
-   - eassumption.
    - destructAll. do 2 eexists. split. eassumption.
      split.
      split. intros. split. eassumption. eassumption. eassumption.
@@ -66,6 +65,47 @@ Section Inline.
  Qed.
 
 End Inline.
+
+
+Section LambdaLift.
+  
+  Lemma lambda_lift_correct e c k l b :
+   well_scoped e ->
+   max_var e 1 < state.next_var c ->
+   exists (e' : exp) (c' : state.comp_data),
+     lambda_lift e k l b c = (Ret e', c') /\
+     max_var e' 1 < state.next_var c' /\
+     wf_pres e e' /\
+     (forall (k : nat) (rho1 rho2 : env),
+         preord_env_P cenv (ll_bound 0) (occurs_free e) k rho1 rho2 ->
+         binding_in_map (occurs_free e) rho1 ->
+         preord_exp cenv (ll_bound 0) (ll_bound 0) k (e, rho1) (e', rho2)).
+  Proof.
+    intros.
+   edestruct lambda_lift_correct_top with (P1 := ll_bound)
+                                          (PG := ll_bound 0).   
+    - intros. eapply ll_bound_compat.
+    - intros. eapply ll_bound_compat.
+      exact (M.empty _). exact 0%nat.
+    - eapply ll_bound_mon. omega.
+    - intros. eapply ll_bound_local_steps; eauto.
+    - intros. eapply ll_bound_local_app.
+    - intros. eapply ll_bound_local_steps_let_app; eauto.
+    - intros. eapply ll_bound_local_steps_let_app_OOT; eauto.
+    - intros. eapply ll_bound_local_steps_app; eauto.
+    - intros. eapply ll_bound_ctx_r; eauto.
+    - eapply H.
+    - eassumption.
+    - eapply H. 
+    - destructAll. do 2 eexists. split. eassumption.
+      split. eassumption.
+      split. intros. split.
+      intros. inv H7. split. eassumption. eassumption. eassumption.
+      eassumption.
+ Qed.
+   
+End LambdaLift.
+  
 
 Section CCHoist.
 
